%!TEX root = ../thesis.tex

\appendix
\section{\texorpdfstring{$3|1$}{3|1}-dimensionaalse
    \texorpdfstring{$3$}{3}-Lie superalgebra kommutatsiooniseosed
}\label{lisa:3|1 kommutatsiooniseosed}

\begin{enumerate}
    \item $\begin{matrix*}[l]
            & [e_1, e_2, e_3] = 2 c_{5} e_1 - 2 c_{4} e_2 + 2 c_{3} e_3, \\
            & [e_1, e_2, f_1] = c_{3} f_1, \\
            & [e_1, e_3, f_1] = c_{4} f_1, \\
            & [e_2, e_3, f_1] = c_{5} f_1, \\
            & [e_1, f_1, f_1] = \left(-c_{1} - c_{2}\right) e_1 + \frac{c_{1} c_{4} + c_{2} c_{4}}{c_{5}} e_2 + \frac{-c_{1} c_{3} - c_{2} c_{3}}{c_{5}} e_3, \\
            & [e_2, f_1, f_1] = -\frac{c_{2} c_{5}}{c_{4}} e_1 + c_{2} e_2 - \frac{c_{2} c_{3}}{c_{4}} e_3, \\
            & [e_3, f_1, f_1] = \frac{c_{1} c_{5}}{c_{3}} e_1 - \frac{c_{1} c_{4}}{c_{3}} e_2 + c_{1} e_3, \\
        \end{matrix*}$

    \item $\begin{matrix*}[l]
            & [e_1, e_2, e_3] = \frac{c_{1} c_{4}}{c_{2}} e_1 - \frac{c_{1} c_{3}}{c_{2}} e_2 + c_{1} e_3, \\
            & [e_1, e_2, f_1] = c_{2} f_1, \\
            & [e_1, e_3, f_1] = c_{3} f_1, \\
            & [e_2, e_3, f_1] = c_{4} f_1, \\
        \end{matrix*}$

    \item $\begin{matrix*}[l]
            & [e_1, e_2, e_3] = 2 c_{4} e_1 - 2 c_{3} e_2 + 2 c_{2} e_3, \\
            & [e_1, e_2, f_1] = c_{2} f_1, \\
            & [e_1, e_3, f_1] = c_{3} f_1, \\
            & [e_2, e_3, f_1] = c_{4} f_1, \\
            & [e_1, f_1, f_1] = -c_{1} e_1 + \frac{c_{1} c_{3}}{c_{4}} e_2 - \frac{c_{1} c_{2}}{c_{4}} e_3, \\
            & [e_3, f_1, f_1] = \frac{c_{1} c_{4}}{c_{2}} e_1 - \frac{c_{1} c_{3}}{c_{2}} e_2 + c_{1} e_3, \\
        \end{matrix*}$

    \item $\begin{matrix*}[l]
            & [e_1, e_2, e_3] = 2 c_{4} e_1 - 2 c_{3} e_2 + 2 c_{2} e_3, \\
            & [e_1, e_2, f_1] = c_{2} f_1, \\
            & [e_1, e_3, f_1] = c_{3} f_1, \\
            & [e_2, e_3, f_1] = c_{4} f_1, \\
            & [e_2, f_1, f_1] = \frac{c_{1} c_{4}}{c_{3}} e_1 - c_{1} e_2 + \frac{c_{1} c_{2}}{c_{3}} e_3, \\
            & [e_3, f_1, f_1] = \frac{c_{1} c_{4}}{c_{2}} e_1 - \frac{c_{1} c_{3}}{c_{2}} e_2 + c_{1} e_3, \\
        \end{matrix*}$

    \item $\begin{matrix*}[l]
            & [e_1, e_2, e_3] = 2 c_{4} e_1 - 2 c_{3} e_2 , \\
            & [e_1, e_3, f_1] = c_{3} f_1, \\
            & [e_2, e_3, f_1] = c_{4} f_1, \\
            & [e_1, f_1, f_1] = -c_{2} e_1 + \frac{c_{2} c_{3}}{c_{4}} e_2 , \\
            & [e_2, f_1, f_1] = -\frac{c_{2} c_{4}}{c_{3}} e_1 + c_{2} e_2 , \\
            & [e_3, f_1, f_1] = c_{1} e_1 - \frac{c_{1} c_{3}}{c_{4}} e_2 , \\
        \end{matrix*}$

    \item $\begin{matrix*}[l]
            & [e_1, f_1, f_1] = \left(-c_{1} - c_{3}\right) e_1 + \frac{c_{2} c_{3}}{c_{4}} e_2 + c_{2} e_3, \\
            & [e_2, f_1, f_1] = \frac{-c_{1} c_{4} - c_{3} c_{4}}{c_{2}} e_1 + c_{3} e_2 + c_{4} e_3, \\
            & [e_3, f_1, f_1] = \frac{-c_{1}^2 - c_{1} c_{3}}{c_{2}} e_1 + \frac{c_{1} c_{3}}{c_{4}} e_2 + c_{1} e_3, \\
        \end{matrix*}$
\end{enumerate}

\begin{adjustwidth*}{-0.5cm}{0cm}
\begin{multicols*}{2}
\begin{enumerate}
    \setcounter{enumi}{6}
    \item $\begin{matrix*}[l]
            & [e_1, e_2, e_3] = 2 c_{4} e_1  + 2 c_{3} e_3, \\
            & [e_1, e_2, f_1] = c_{3} f_1, \\
            & [e_2, e_3, f_1] = c_{4} f_1, \\
            & [e_1, f_1, f_1] = c_{1} e_1  + \frac{c_{1} c_{3}}{c_{4}} e_3, \\
            & [e_2, f_1, f_1] = \frac{c_{2} c_{4}}{c_{3}} e_1  + c_{2} e_3, \\
            & [e_3, f_1, f_1] = -\frac{c_{1} c_{4}}{c_{3}} e_1  - c_{1} e_3, \\
        \end{matrix*}$

    \item $\begin{matrix*}[l]
            & [e_1, e_2, e_3] = 2 c_{4} e_1  + 2 c_{3} e_3, \\
            & [e_1, e_2, f_1] = c_{3} f_1, \\
            & [e_2, e_3, f_1] = c_{4} f_1, \\
            & [e_1, f_1, f_1] = -c_{1} e_1  - \frac{c_{1} c_{3}}{c_{4}} e_3, \\
            & [e_2, f_1, f_1] = \frac{c_{2} c_{4}}{c_{3}} e_1  + c_{2} e_3, \\
            & [e_3, f_1, f_1] = \frac{c_{1} c_{4}}{c_{3}} e_1  + c_{1} e_3, \\
        \end{matrix*}$

    \item $\begin{matrix*}[l]
            & [e_1, e_2, e_3] =  - 2 c_{4} e_2 + 2 c_{3} e_3, \\
            & [e_1, e_2, f_1] = c_{3} f_1, \\
            & [e_1, e_3, f_1] = c_{4} f_1, \\
            & [e_1, f_1, f_1] =  - \frac{c_{1} c_{4}}{c_{3}} e_2 + c_{1} e_3, \\
            & [e_2, f_1, f_1] =  c_{2} e_2 - \frac{c_{2} c_{3}}{c_{4}} e_3, \\
            & [e_3, f_1, f_1] =  \frac{c_{2} c_{4}}{c_{3}} e_2 - c_{2} e_3, \\
        \end{matrix*}$

    \item $\begin{matrix*}[l]
            & [e_1, e_2, e_3] =  - 2 c_{4} e_2 + 2 c_{3} e_3, \\
            & [e_1, e_2, f_1] = c_{3} f_1, \\
            & [e_1, e_3, f_1] = c_{4} f_1, \\
            & [e_1, f_1, f_1] =  - \frac{c_{2} c_{4}}{c_{3}} e_2 + c_{2} e_3, \\
            & [e_2, f_1, f_1] =  - c_{1} e_2 + \frac{c_{1} c_{3}}{c_{4}} e_3, \\
            & [e_3, f_1, f_1] =  - \frac{c_{1} c_{4}}{c_{3}} e_2 + c_{1} e_3, \\
        \end{matrix*}$

    \item $\begin{matrix*}[l]
            & [e_1, e_2, e_3] = 2 c_{3} e_1 - 2 c_{2} e_2 + 2 c_{1} e_3, \\
            & [e_1, e_2, f_1] = c_{1} f_1, \\
            & [e_1, e_3, f_1] = c_{2} f_1, \\
            & [e_2, e_3, f_1] = c_{3} f_1, \\
        \end{matrix*}$

    \item $\begin{matrix*}[l]
            & [e_1, e_2, e_3] = c_{1} e_1 - \frac{c_{1} c_{2}}{c_{3}} e_2 , \\
            & [e_1, e_3, f_1] = c_{2} f_1, \\
            & [e_2, e_3, f_1] = c_{3} f_1, \\
        \end{matrix*}$

    \item $\begin{matrix*}[l]
            & [e_1, e_2, e_3] = 2 c_{3} e_1 - 2 c_{2} e_2 , \\
            & [e_1, e_3, f_1] = c_{2} f_1, \\
            & [e_2, e_3, f_1] = c_{3} f_1, \\
            & [e_3, f_1, f_1] = c_{1} e_1 - \frac{c_{1} c_{2}}{c_{3}} e_2 , \\
        \end{matrix*}$

    \item $\begin{matrix*}[l]
            & [e_1, e_2, e_3] = 2 c_{3} e_1  , \\
            & [e_2, e_3, f_1] = c_{3} f_1, \\
            & [e_2, f_1, f_1] = c_{2} e_1  , \\
            & [e_3, f_1, f_1] = c_{1} e_1  , \\
        \end{matrix*}$

    \item $\begin{matrix*}[l]
            & [e_1, e_2, e_3] =  - 2 c_{3} e_2 , \\
            & [e_1, e_3, f_1] = c_{3} f_1, \\
            & [e_1, f_1, f_1] =  c_{2} e_2 , \\
            & [e_3, f_1, f_1] =  c_{1} e_2 , \\
        \end{matrix*}$

    \item $\begin{matrix*}[l]
            & [e_1, f_1, f_1] = -c_{3} e_1 - \frac{c_{3}^2}{c_{2}} e_2 , \\
            & [e_2, f_1, f_1] = c_{2} e_1 + c_{3} e_2 , \\
            & [e_3, f_1, f_1] = c_{1} e_1 + \frac{c_{1} c_{3}}{c_{2}} e_2 , \\
        \end{matrix*}$

    \item $\begin{matrix*}[l]
            & [e_1, f_1, f_1] =  \frac{c_{1} c_{2}}{c_{3}} e_2 + c_{1} e_3, \\
            & [e_2, f_1, f_1] =  c_{2} e_2 + c_{3} e_3, \\
            & [e_3, f_1, f_1] =  - \frac{c_{2}^2}{c_{3}} e_2 - c_{2} e_3, \\
        \end{matrix*}$

    \item $\begin{matrix*}[l]
            & [e_1, e_2, e_3] = c_{1} e_1 + c_{2} e_2 + c_{3} e_3, \\
        \end{matrix*}$

    \item $\begin{matrix*}[l]
            & [e_1, f_1, f_1] = -c_{1} e_1 + c_{2} e_2 + c_{3} e_3, \\
            & [e_3, f_1, f_1] = -\frac{c_{1}^2}{c_{3}} e_1 + \frac{c_{1} c_{2}}{c_{3}} e_2 + c_{1} e_3, \\
        \end{matrix*}$

    \item $\begin{matrix*}[l]
            & [e_2, f_1, f_1] = c_{2} e_1 - c_{1} e_2 + c_{3} e_3, \\
            & [e_3, f_1, f_1] = \frac{c_{1} c_{2}}{c_{3}} e_1 - \frac{c_{1}^2}{c_{3}} e_2 + c_{1} e_3, \\
        \end{matrix*}$

    \item $\begin{matrix*}[l]
            & [e_1, f_1, f_1] =  - \frac{c_{1} c_{2}}{c_{3}} e_2 + c_{2} e_3, \\
            & [e_2, f_1, f_1] =  - c_{1} e_2 + c_{3} e_3, \\
            & [e_3, f_1, f_1] =  - \frac{c_{1}^2}{c_{3}} e_2 + c_{1} e_3, \\
        \end{matrix*}$

    \item $\begin{matrix*}[l]
            & [e_1, e_2, e_3] = 2 c_{3} e_1  + 2 c_{2} e_3, \\
            & [e_1, e_2, f_1] = c_{2} f_1, \\
            & [e_2, e_3, f_1] = c_{3} f_1, \\
            & [e_1, f_1, f_1] =  0, e_2 , \\
            & [e_2, f_1, f_1] = \frac{c_{1} c_{3}}{c_{2}} e_1  + c_{1} e_3, \\
        \end{matrix*}$

    \item $\begin{matrix*}[l]
            & [e_1, e_2, e_3] = \frac{c_{1} c_{3}}{c_{2}} e_1  + c_{1} e_3, \\
            & [e_1, e_2, f_1] = c_{2} f_1, \\
            & [e_2, e_3, f_1] = c_{3} f_1, \\
        \end{matrix*}$

    \item $\begin{matrix*}[l]
            & [e_1, e_2, e_3] = 2 c_{3} e_1  + 2 c_{2} e_3, \\
            & [e_1, e_2, f_1] = c_{2} f_1, \\
            & [e_2, e_3, f_1] = c_{3} f_1, \\
            & [e_1, f_1, f_1] = -c_{1} e_1  - \frac{c_{1} c_{2}}{c_{3}} e_3, \\
            & [e_3, f_1, f_1] = \frac{c_{1} c_{3}}{c_{2}} e_1  + c_{1} e_3, \\
        \end{matrix*}$

    \item $\begin{matrix*}[l]
            & [e_1, f_1, f_1] = c_{1} e_1  + c_{2} e_3, \\
            & [e_2, f_1, f_1] = \frac{c_{1} c_{3}}{c_{2}} e_1  + c_{3} e_3, \\
            & [e_3, f_1, f_1] = -\frac{c_{1}^2}{c_{2}} e_1  - c_{1} e_3, \\
        \end{matrix*}$

    \item $\begin{matrix*}[l]
            & [e_1, e_2, e_3] =  2 c_{3} e_3, \\
            & [e_1, e_2, f_1] = c_{3} f_1, \\
            & [e_1, f_1, f_1] =  c_{1} e_3, \\
            & [e_2, f_1, f_1] =  c_{2} e_3, \\
        \end{matrix*}$

    \item $\begin{matrix*}[l]
            & [e_1, e_2, e_3] =  - 2 c_{3} e_2 + 2 c_{2} e_3, \\
            & [e_1, e_2, f_1] = c_{2} f_1, \\
            & [e_1, e_3, f_1] = c_{3} f_1, \\
            & [e_1, f_1, f_1] =  - \frac{c_{1} c_{3}}{c_{2}} e_2 + c_{1} e_3, \\
        \end{matrix*}$

    \item $\begin{matrix*}[l]
            & [e_1, e_2, e_3] =  - 2 c_{3} e_2 + 2 c_{2} e_3, \\
            & [e_1, e_2, f_1] = c_{2} f_1, \\
            & [e_1, e_3, f_1] = c_{3} f_1, \\
            & [e_2, f_1, f_1] =  c_{1} e_2 - \frac{c_{1} c_{2}}{c_{3}} e_3, \\
            & [e_3, f_1, f_1] =  \frac{c_{1} c_{3}}{c_{2}} e_2 - c_{1} e_3, \\
        \end{matrix*}$

    \item $\begin{matrix*}[l]
            & [e_1, e_2, e_3] =  c_{1} e_2 - \frac{c_{1} c_{2}}{c_{3}} e_3, \\
            & [e_1, e_2, f_1] = c_{2} f_1, \\
            & [e_1, e_3, f_1] = c_{3} f_1, \\
        \end{matrix*}$

    \item $\begin{matrix*}[l]
            & [e_1, e_2, e_3] =  - 2 c_{3} e_2 + 2 c_{2} e_3, \\
            & [e_1, e_2, f_1] = c_{2} f_1, \\
            & [e_1, e_3, f_1] = c_{3} f_1, \\
            & [e_2, f_1, f_1] =  - c_{1} e_2 + \frac{c_{1} c_{2}}{c_{3}} e_3, \\
            & [e_3, f_1, f_1] =  - \frac{c_{1} c_{3}}{c_{2}} e_2 + c_{1} e_3, \\
        \end{matrix*}$

    \item $\begin{matrix*}[l]
            & [e_1, e_3, f_1] = c_{1} f_1, \\
            & [e_2, e_3, f_1] = c_{2} f_1, \\
        \end{matrix*}$

    \item $\begin{matrix*}[l]
            & [e_1, e_2, e_3] = 2 c_{2} e_1 - 2 c_{1} e_2 , \\
            & [e_1, e_3, f_1] = c_{1} f_1, \\
            & [e_2, e_3, f_1] = c_{2} f_1, \\
        \end{matrix*}$

    \item $\begin{matrix*}[l]
            & [e_1, e_2, e_3] = c_{1} e_1  , \\
            & [e_2, e_3, f_1] = c_{2} f_1, \\
        \end{matrix*}$

    \item $\begin{matrix*}[l]
            & [e_1, e_2, e_3] =  c_{1} e_2 , \\
            & [e_1, e_3, f_1] = c_{2} f_1, \\
        \end{matrix*}$

    \item $\begin{matrix*}[l]
            & [e_2, f_1, f_1] = c_{1} e_1  + c_{2} e_3, \\
        \end{matrix*}$

    \item $\begin{matrix*}[l]
            & [e_2, f_1, f_1] = c_{2} e_1  , \\
            & [e_3, f_1, f_1] = c_{1} e_1  , \\
        \end{matrix*}$

    \item $\begin{matrix*}[l]
            & [e_1, f_1, f_1] =  c_{2} e_2 , \\
            & [e_3, f_1, f_1] =  c_{1} e_2 , \\
        \end{matrix*}$

    \item $\begin{matrix*}[l]
            & [e_3, f_1, f_1] = c_{1} e_1 + c_{2} e_2 , \\
        \end{matrix*}$

    \item $\begin{matrix*}[l]
            & [e_1, f_1, f_1] =  c_{1} e_2 + c_{2} e_3, \\
        \end{matrix*}$

    \item $\begin{matrix*}[l]
            & [e_2, f_1, f_1] =  c_{1} e_2 + c_{2} e_3, \\
            & [e_3, f_1, f_1] =  - \frac{c_{1}^2}{c_{2}} e_2 - c_{1} e_3, \\
        \end{matrix*}$

    \item $\begin{matrix*}[l]
            & [e_1, e_2, e_3] = c_{1} e_1  + c_{2} e_3, \\
        \end{matrix*}$

    \item $\begin{matrix*}[l]
            & [e_1, f_1, f_1] =  c_{1} e_3, \\
            & [e_2, f_1, f_1] =  c_{2} e_3, \\
        \end{matrix*}$

    \item $\begin{matrix*}[l]
            & [e_2, f_1, f_1] =  - c_{1} e_2 + c_{2} e_3, \\
            & [e_3, f_1, f_1] =  - \frac{c_{1}^2}{c_{2}} e_2 + c_{1} e_3, \\
        \end{matrix*}$

    \item $\begin{matrix*}[l]
            & [e_1, e_2, e_3] = 2 c_{2} e_1  + 2 c_{1} e_3, \\
            & [e_1, e_2, f_1] = c_{1} f_1, \\
            & [e_2, e_3, f_1] = c_{2} f_1, \\
            & [e_1, f_1, f_1] =  0, e_2 , \\
        \end{matrix*}$

    \item $\begin{matrix*}[l]
            & [e_1, e_2, f_1] = c_{1} f_1, \\
            & [e_2, e_3, f_1] = c_{2} f_1, \\
        \end{matrix*}$

    \item $\begin{matrix*}[l]
            & [e_1, e_2, e_3] =  c_{1} e_2 + c_{2} e_3, \\
        \end{matrix*}$

    \item $\begin{matrix*}[l]
            & [e_1, e_2, e_3] =  c_{1} e_3, \\
            & [e_1, e_2, f_1] = c_{2} f_1, \\
        \end{matrix*}$

    \item $\begin{matrix*}[l]
            & [e_1, e_2, e_3] =  - 2 c_{2} e_2 + 2 c_{1} e_3, \\
            & [e_1, e_2, f_1] = c_{1} f_1, \\
            & [e_1, e_3, f_1] = c_{2} f_1, \\
        \end{matrix*}$

    \item $\begin{matrix*}[l]
            & [e_1, e_2, f_1] = c_{1} f_1, \\
            & [e_1, e_3, f_1] = c_{2} f_1, \\
        \end{matrix*}$

    \item $\begin{matrix*}[l]
            & [e_1, e_2, e_3] = c_{1} e_1 + c_{2} e_2 , \\
        \end{matrix*}$

    \item $\begin{matrix*}[l]
            & [e_2, e_3, f_1] = c_{1} f_1, \\
        \end{matrix*}$

    \item $\begin{matrix*}[l]
            & [e_1, e_2, e_3] =  c_{1} e_3, \\
        \end{matrix*}$

    \item $\begin{matrix*}[l]
            & [e_2, f_1, f_1] =  c_{1} e_3, \\
        \end{matrix*}$

    \item $\begin{matrix*}[l]
            & [e_1, e_2, e_3] = c_{1} e_1  , \\
        \end{matrix*}$

    \item $\begin{matrix*}[l]
            & [e_1, e_2, e_3] =  c_{1} e_2 , \\
        \end{matrix*}$
\end{enumerate}
\end{multicols*}
\end{adjustwidth*}
